\documentclass{article}
\usepackage{zed-cm}
\usepackage{zed-maths}
\usepackage{zed-proof}
\usepackage{amsmath}
\begin{document}

\section*{Propositional Logic}

\bigskip
\noindent
\textbf{Solution 1}

\medskip

\bigskip
\noindent
\textbf{Solution 2}

\medskip

(a)
\par
\vspace{11pt}
\begin{center}
\begin{tabular}{c c c c}
$p$ & $q$ & $p \land q$ & $( p \land q ) \Rightarrow p$ \\
\hline
t & t & t & t \\
t & f & f & t \\
f & t & f & t \\
f & f & f & t \\
\end{tabular}
\end{center}

\begin{center}
\begin{tabular}{c c c c c}
$p$ & $q$ & $p \land q$ & $\lnot p$ & $\lnot p \Rightarrow ( p \land q )$ \\
\hline
t & t & t & f & t \\
t & f & f & f & t \\
f & t & f & t & f \\
f & f & f & t & f \\
\end{tabular}
\end{center}

\begin{center}
\begin{tabular}{c c c c c}
$p$ & $q$ & $p \Rightarrow q$ & $p \land ( p \Rightarrow q )$ & $( \lnot p \Rightarrow ( p \land q ) ) \Leftrightarrow p$ \\
\hline
t & t & t & t & t \\
t & f & f & f & t \\
f & t & t & f & t \\
f & f & t & f & t \\
\end{tabular}
\end{center}

\medskip

(b)
\par
\vspace{11pt}
\begin{center}
\begin{tabular}{c c c c c}
$p$ & $q$ & $p \Rightarrow q$ & $p \land ( p \Rightarrow q )$ & $( p \land ( p \Rightarrow q ) ) \Rightarrow q$ \\
\hline
t & t & t & t & t \\
t & f & f & f & t \\
f & t & t & f & t \\
f & f & t & f & t \\
\end{tabular}
\end{center}

\medskip

\bigskip
\noindent
\textbf{Solution 3}

\medskip

(a)
\par
\vspace{11pt}
\vspace{-10pt}
\begin{align*}
p \Rightarrow \lnot p \\
&\Leftrightarrow \lnot p \lor \lnot p && \text{[$\Rightarrow$]} \\
&\Leftrightarrow \lnot p && \text{[idempotence]}
\end{align*}

\medskip

(b)
\par
\vspace{11pt}
\vspace{-10pt}
\begin{align*}
\lnot p \Rightarrow p \\
&\Leftrightarrow \lnot \lnot p \lor p && \text{[$\Rightarrow$]} \\
&\Leftrightarrow p \lor p && \text{[$\lnot$ $\lnot$]} \\
&\Leftrightarrow p && \text{[idempotence]}
\end{align*}

\medskip

(c)
\par
\vspace{11pt}
\vspace{-10pt}
\begin{align*}
p \Rightarrow q \Rightarrow r \\
&\Leftrightarrow \lnot p \lor (q \Rightarrow r) && \text{[$\Rightarrow$]} \\
&\Leftrightarrow \lnot p \lor \lnot q \lor r && \text{[$\Rightarrow$]} \\
&\Leftrightarrow \lnot p \lor \lnot q \lor r && \text{[associativity]} \\
&\Leftrightarrow \lnot p \land q \lor r && \text{[De Morgan]} \\
&\Leftrightarrow p \land q \Rightarrow r && \text{[$\Rightarrow$]}
\end{align*}

\medskip

(d)
\par
\vspace{11pt}
\vspace{-10pt}
\begin{align*}
q \Rightarrow p \Rightarrow r \\
&\Leftrightarrow \lnot q \lor (p \Rightarrow r) && \text{[$\Rightarrow$]} \\
&\Leftrightarrow \lnot q \lor \lnot p \lor r && \text{[$\Rightarrow$]} \\
&\Leftrightarrow \lnot p \lor \lnot q \lor r && \text{[associativity $\land$ commutativity]} \\
&\Leftrightarrow \lnot p \lor (q \Rightarrow r) && \text{[$\Rightarrow$]} \\
&\Leftrightarrow p \Rightarrow q \Rightarrow r && \text{[$\Rightarrow$]}
\end{align*}

\medskip

(e)
\par
\vspace{11pt}
\vspace{-10pt}
\begin{align*}
p \land q \Leftrightarrow p \\
&\Leftrightarrow (p \land q \Rightarrow p) \land (p \Rightarrow p \land q) && \text{[$\Leftrightarrow$]} \\
&\Leftrightarrow (\lnot p \land q \lor p) \land (\lnot p \lor p \land q) && \text{[$\Rightarrow$]} \\
&\Leftrightarrow (\lnot p \lor \lnot q \lor p) \land (\lnot p \lor p \land q) && \text{[De Morgan]} \\
&\Leftrightarrow (\lnot q \lor \lnot p \lor p) \land (\lnot p \lor p \land q) && \text{[associativity $\land$ comm]} \\
&\Leftrightarrow (\lnot q \lor true) \land (\lnot p \lor p \land q) && \text{[excluded middle]} \\
&\Leftrightarrow true \land (\lnot p \lor p \land q) && \text{[$\lor$ $\land$ true]} \\
&\Leftrightarrow \lnot p \lor p \land q && \text{[$\land$ $\land$ true]} \\
&\Leftrightarrow (\lnot p \lor p) \land (\lnot p \lor q) && \text{[distribution]} \\
&\Leftrightarrow true \land (\lnot p \lor q) && \text{[excluded middle]} \\
&\Leftrightarrow \lnot p \lor q && \text{[$\land$ $\land$ true]} \\
&\Leftrightarrow p \Rightarrow q && \text{[$\Rightarrow$]}
\end{align*}

\medskip

(f)
\par
\vspace{11pt}
\vspace{-10pt}
\begin{align*}
p \lor q \Leftrightarrow p \\
&\Leftrightarrow (p \lor q \Rightarrow p) \land (p \Rightarrow p \lor q) && \text{[$\Leftrightarrow$]} \\
&\Leftrightarrow (\lnot p \lor q \lor p) \land (\lnot p \lor p \lor q) && \text{[$\Rightarrow$]} \\
&\Leftrightarrow (\lnot p \land \lnot q \lor p) \land (\lnot p \lor p \lor q) && \text{[De Morgan]} \\
&\Leftrightarrow (\lnot p \lor p) \land (\lnot q \lor p) \land (\lnot p \lor p \lor q) && \text{[distribution]} \\
&\Leftrightarrow true \land (\lnot q \lor p) \land (\lnot p \lor p \lor q) && \text{[excluded middle]} \\
&\Leftrightarrow (\lnot q \lor p) \land (\lnot p \lor p \lor q) && \text{[$\land$ $\land$ true]} \\
&\Leftrightarrow (\lnot q \lor p) \land (\lnot p \lor p \lor q) && \text{[associativity]} \\
&\Leftrightarrow (\lnot q \lor p) \land (true \lor q) && \text{[excluded middle]} \\
&\Leftrightarrow (\lnot q \lor p) \land true && \text{[$\lor$ $\land$ true]} \\
&\Leftrightarrow \lnot q \lor p && \text{[$\land$ $\land$ true]} \\
&\Leftrightarrow q \Rightarrow p && \text{[$\Rightarrow$]}
\end{align*}

\medskip

\bigskip
\noindent
\textbf{Solution 4}

\medskip

\bigskip
\noindent
\textbf{Solution 5}

\medskip

\bigskip
\noindent
\textbf{Solution 6}

\medskip

\bigskip
\noindent
\textbf{Solution 7}

\medskip

\bigskip
\noindent
\textbf{Solution 8}

\medskip

\section*{Equality}

\bigskip
\noindent
\textbf{Solution 9}

\medskip

\bigskip
\noindent
\textbf{Solution 10}

\medskip

\bigskip
\noindent
\textbf{Solution 11}

\medskip

\bigskip
\noindent
\textbf{Solution 12}

\medskip

\section*{Deductive Proofs}

\bigskip
\noindent
\textbf{Solution 13}

\medskip

\vspace{13pt}
\noindent
\infer[$\Rightarrow$\text{-intro}^{[1]}]{p \land (p \Rightarrow q) \Rightarrow p \land q}{
  \infer[\text{$\land$ intro}]{p \land q}{\infer[\text{$\Rightarrow$ elim}]{q}{\infer[$\land$\text{-elim-1}]{p}{\ulcorner p \land (p \Rightarrow q) \urcorner^{[1]}} & \infer[$\land$\text{-elim-2}]{p \Rightarrow q}{\ulcorner p \land (p \Rightarrow q) \urcorner^{[1]}}}}
}

\bigskip
\noindent
\textbf{Solution 14}

\medskip

\vspace{13pt}
\noindent
\infer[$\Rightarrow$\text{-intro}^{[1]}]{(p \land q \Leftrightarrow p) \Rightarrow p \Rightarrow q}{
  \infer[$\Rightarrow$\text{-intro}^{[2]}]{p \Rightarrow q}{\infer[\text{assumption}]{p}{\infer[\text{$\Rightarrow$ elim}]{p \land q}{} & \infer[$\land$\text{-elim-2}]{q}{}}}
}

\vspace{13pt}
\noindent
\infer[$\Rightarrow$\text{-intro}^{[1]}]{p \Rightarrow q \Rightarrow (p \land q \Leftrightarrow p)}{
  \infer[\text{$\Leftrightarrow$ intro}]{p \land q \Leftrightarrow p}{\infer[$\Rightarrow$\text{-intro}^{[3]}]{p \Rightarrow p \land q}{\infer[\text{$\land$ intro}]{p \land q}{\infer[\text{$\Rightarrow$ elim}]{q}{\ulcorner p \urcorner^{[3]}}}}}
}

\bigskip
\noindent
\textbf{Solution 15}

\medskip

\vspace{13pt}
\noindent
\infer[$\Rightarrow$\text{-intro}^{[1]}]{(p \Rightarrow q) \land \lnot q \Rightarrow \lnot p}{
  \infer[negation\text{-intro}^{[2]}]{\lnot p}{\infer[$\land$\text{-elim-1}]{p \Rightarrow q}{\ulcorner (p \Rightarrow q) \land \lnot q \urcorner^{[1]}} & \infer[$\land$\text{-elim-2}]{\lnot q}{\ulcorner (p \Rightarrow q) \land \lnot q \urcorner^{[1]}} & \infer[\text{contradiction}]{false}{\infer[\text{$\Rightarrow$ elim}]{q}{\ulcorner p \urcorner^{[2]}}}}
}

\bigskip
\noindent
\textbf{Solution 16}

\medskip

\vspace{13pt}
\noindent
\infer[$\Rightarrow$\text{-intro}^{[1]}]{p \land (q \lor r) \Rightarrow p \land q \lor p \land r}{
  \infer[$\lor$\text{-elim}^{[2]}]{p \land q \lor p \land r}{\infer[$\land$\text{-elim-2}]{q \lor r}{\ulcorner p \land (q \lor r) \urcorner^{[1]}} & \raiseproof{12ex}{\infer[$\lor$\text{-intro-1}]{p \land q \lor p \land r}{\infer[\text{$\land$ intro}]{p \land q}{\infer[\text{from above}]{p}{} & \infer[\text{from case}]{q}{}}}} & \hskip 6em \raiseproof{30ex}{\infer[$\lor$\text{-intro-2}]{p \land q \lor p \land r}{\infer[\text{$\land$ intro}]{p \land r}{\infer[\text{from above}]{p}{} & \infer[\text{from case}]{r}{}}}}}
}

\vspace{13pt}
\noindent
\infer[$\Rightarrow$\text{-intro}^{[3]}]{p \land q \lor p \land r \Rightarrow p \land (q \lor r)}{
  \infer[$\lor$\text{-elim}^{[4]}]{p \land (q \lor r)}{\infer[\text{$\land$ intro}]{p \land (q \lor r)}{\infer[$\lor$\text{-intro-1}]{q \lor r}{\infer[$\land$\text{-elim-1}]{p}{\ulcorner p \land q \urcorner^{[4]}} & \infer[$\land$\text{-elim-2}]{q}{\ulcorner p \land q \urcorner^{[4]}}}} & \infer[\text{$\land$ intro}]{p \land (q \lor r)}{\infer[$\lor$\text{-intro-2}]{q \lor r}{\infer[$\land$\text{-elim-1}]{p}{\ulcorner p \land r \urcorner^{[4]}} & \infer[$\land$\text{-elim-2}]{r}{\ulcorner p \land r \urcorner^{[4]}}}}}
}

\bigskip
\noindent
\textbf{Solution 17}

\medskip

\vspace{13pt}
\noindent
\infer[$\Rightarrow$\text{-intro}^{[3]}]{p \lor q \land r \Rightarrow (p \lor q) \land (p \lor r)}{
  \infer[$\lor$\text{-elim}^{[1]}]{(p \lor q) \land (p \lor r)}{\infer[\text{$\land$ intro}]{(p \lor q) \land (p \lor r)}{\infer[$\lor$\text{-intro-1}]{p \lor q}{\ulcorner p \urcorner^{[1]}} & \infer[$\lor$\text{-intro-1}]{p \lor r}{\ulcorner p \urcorner^{[1]}}} & \infer[\text{$\land$ intro}]{(p \lor q) \land (p \lor r)}{\infer[$\land$\text{-elim-1}]{q}{\ulcorner q \land r \urcorner^{[1]}} & \infer[$\land$\text{-elim-2}]{r}{\ulcorner q \land r \urcorner^{[1]}} & \infer[$\lor$\text{-intro-2}]{p \lor q}{\ulcorner q \land r \urcorner^{[1]}} & \infer[$\lor$\text{-intro-2}]{p \lor r}{\ulcorner q \land r \urcorner^{[1]}}}}
}

\vspace{13pt}
\noindent
\infer[$\Rightarrow$\text{-intro}^{[1]}]{(p \lor q) \land (p \lor r) \Rightarrow p \lor q \land r}{
  \infer[$\lor$\text{-elim}^{[2]}]{p \lor q \land r}{\infer[$\land$\text{-elim-1}]{p \lor q}{\ulcorner (p \lor q) \land (p \lor r) \urcorner^{[1]}} & \infer[$\land$\text{-elim-2}]{p \lor r}{\ulcorner (p \lor q) \land (p \lor r) \urcorner^{[1]}} & \raiseproof{10ex}{\infer[$\lor$\text{-intro-1}]{p \lor q \land r}{\ulcorner p \urcorner^{[2]}}} & \hskip 6em \raiseproof{38ex}{\infer[$\lor$\text{-elim}^{[3]}]{p \lor q \land r}{\infer[$\lor$\text{-intro-1}]{p \lor q \land r}{\ulcorner p \urcorner^{[3]}} & \infer[$\lor$\text{-intro-2}]{p \lor q \land r}{\infer[\text{$\land$ intro}]{q \land r}{\ulcorner r \urcorner^{[3]}}}}}}
}

\bigskip
\noindent
\textbf{Solution 18}

\medskip

\vspace{13pt}
\noindent
\infer[$\Rightarrow$\text{-intro}^{[1]}]{p \Rightarrow q \Rightarrow \lnot p \lor q}{
  \infer[\text{excluded middle}]{p \lor \lnot p}{\ulcorner p \Rightarrow q \urcorner^{[1]}} & \infer[$\lor$\text{-elim}^{[2]}]{\lnot p \lor q}{\infer[$\lor$\text{-intro-2}]{\lnot p \lor q}{\infer[\text{$\Rightarrow$ elim}]{q}{\ulcorner p \urcorner^{[2]}}} & \infer[$\lor$\text{-intro-1}]{\lnot p \lor q}{\ulcorner \lnot p \urcorner^{[2]}}}
}

\vspace{13pt}
\noindent
\infer[$\Rightarrow$\text{-intro}^{[3]}]{\lnot p \lor q \Rightarrow p \Rightarrow q}{
  \infer[$\Rightarrow$\text{-intro}^{[4]}]{p \Rightarrow q}{\infer[\text{assumption}]{p}{\infer[$\lor$\text{-elim}^{[5]}]{q}{\infer[\text{false elim}]{q}{\infer[\text{contradiction}]{false}{\ulcorner \lnot p \urcorner^{[5]}}} & \ulcorner q \urcorner^{[5]}}}}
}

\section*{Sets and Types}

\bigskip
\noindent
\textbf{Solution 19}

\medskip

\bigskip
\noindent
\textbf{Solution 20}

\medskip

\bigskip
\noindent
\textbf{Solution 21}

\medskip

\bigskip
\noindent
\textbf{Solution 22}

\medskip

\bigskip
\noindent
\textbf{Solution 23}

\medskip

\section*{Definitions}

\bigskip
\noindent
\textbf{Solution 24}

\medskip

(a)
\par
\vspace{11pt}
Pairs == Z

$x$

$Z$

\medskip

(b)
\par
\vspace{11pt}
StrictlyPositivePairs == Pairs

\medskip

(c)
\par
\vspace{11pt}
\begin{zed}[Person]\end{zed}

\medskip

(d)
\par
\vspace{11pt}
Couples == Pairs

\medskip

(e)
\par
\vspace{11pt}
Parties == Pairs

\medskip

\bigskip
\noindent
\textbf{Solution 25}

\medskip

\bigskip
\noindent
\textbf{Solution 26}

\medskip

\section*{Relations}

\bigskip
\noindent
\textbf{Solution 27}

\medskip

\bigskip
\noindent
\textbf{Solution 28}

\medskip

\bigskip
\noindent
\textbf{Solution 29}

\medskip

\bigskip
\noindent
\textbf{Solution 30}

\medskip

\bigskip
\noindent
\textbf{Solution 31}

\medskip

\bigskip
\noindent
\textbf{Solution 32}

\medskip

\section*{Functions}

\bigskip
\noindent
\textbf{Solution 33}

\medskip

\bigskip
\noindent
\textbf{Solution 34}

\medskip

\bigskip
\noindent
\textbf{Solution 35}

\medskip

\bigskip
\noindent
\textbf{Solution 36}

\medskip

\section*{Sequences}

\bigskip
\noindent
\textbf{Solution 37}

\medskip

\bigskip
\noindent
\textbf{Solution 38}

\medskip

\bigskip
\noindent
\textbf{Solution 39}

\medskip

\section*{Modelling}

\bigskip
\noindent
\textbf{Solution 40}

\medskip

\bigskip
\noindent
\textbf{Solution 41}

\medskip

\bigskip
\noindent
\textbf{Solution 42}

\medskip

\bigskip
\noindent
\textbf{Solution 43}

\medskip

\section*{Free Types and Induction}

\bigskip
\noindent
\textbf{Solution 44}

\medskip

\bigskip
\noindent
\textbf{Solution 45}

\medskip

\end{document}