\documentclass{article}
\usepackage{zed-cm}
\usepackage{zed-maths}
\usepackage{zed-proof}
\begin{document}

\section*{Test Proof Tree}

$$
\infer[\Rightarrow\text{-intro}]{(p \land (p \Rightarrow q)) \Rightarrow (p \land q)}{
  \infer[\land\text{-intro}]{p \land q}{
    \infer[\land\text{-elim}]{p}{p \land (p \Rightarrow q)}
    &
    \infer[\Rightarrow\text{-elim}]{q}{
      \infer[\land\text{-elim}]{p \Rightarrow q}{p \land (p \Rightarrow q)}
      &
      \infer[\land\text{-elim}]{p}{p \land (p \Rightarrow q)}
    }
  }
}
$$

\end{document}
