\documentclass[a4paper,10pt,fleqn]{article}
\usepackage[margin=1in]{geometry}
\usepackage{amssymb}
\usepackage{natbib}
\usepackage{fuzz}
\usepackage{zed-maths}
\usepackage{zed-proof}
\begin{document}

\section*{One - Point Rule Applications}

\bigskip
\noindent
\textbf{Example 1 : Simple One - Point Rule}

\medskip

\bigskip

When a quantifier binds a variable that is constrained by equality,
we can eliminate the quantifier:

\bigskip

\[
  \begin{array}{ll@{\hspace{2em}}l}
    & \exists y : \nat @ y = 5 \land x > y \\
    &\Leftrightarrow 5 \in \nat \land x > 5 & [\mbox{one - point rule}] \\
    &\Leftrightarrow x > 5
  \end{array}
\]

\bigskip
\noindent
\textbf{Example 2 : One - Point with Set Membership}

\medskip

\[
  \begin{array}{ll@{\hspace{2em}}l}
    & \exists x, y : \nat @ x + y = 4 \land x < y \\
    &\Leftrightarrow \exists x, y : \nat @ y = 4 - x \land x < y \\
    &\Leftrightarrow \exists x : \nat @ 4 - x \in \nat \land x < 4 - x \\
    &\Leftrightarrow true
  \end{array}
\]

\bigskip

The final equivalence holds because $0 \in N$, $4 - 0 \in N$, and 0 $<$ 4.

\bigskip

\bigskip
\noindent
\textbf{Example 3 : One - Point with Disjunction}

\medskip

\[
  \begin{array}{ll@{\hspace{2em}}l}
    & \exists x : \nat @ (x = 1 \land x > y) \lor (x = 2 \land x > z) \\
    &\Leftrightarrow (\exists x : \nat @ x = 1 \land x > y) \lor
    (\exists x : \nat @ x = 2 \land x > z) \\
    &\Leftrightarrow (1 \in \nat \land 1 > y) \lor (\exists x : \nat
    @ x = 2 \land x > z) \\
    &\Leftrightarrow (1 \in \nat \land 1 > y) \lor (2 \in \nat \land 2 > z) \\
    &\Leftrightarrow 1 > y \lor 2 > z
  \end{array}
\]

\bigskip
\noindent
\textbf{Example 4 : One - Point with Expression Part}

\medskip

\[
  \begin{array}{ll@{\hspace{2em}}l}
    & \exists y : \nat @ y = x + 1 \land y > 0 \\
    &\Leftrightarrow x + 1 \in \nat \land x + 1 > 0 & [\mbox{one -
    point rule}] \\
    &\Leftrightarrow x + 1 > 0
  \end{array}
\]

\end{document}
