\documentclass[a4paper,10pt,fleqn]{article}
\usepackage[margin=1in]{geometry}
\usepackage{amssymb}
\usepackage{zed-cm}
\usepackage{zed-maths}
\usepackage{zed-proof}
\begin{document}

\section*{Solution 40 Test ( Conditional Expressions )}

\bigskip
\noindent
\textbf{Solution 40 ( c ) - viewed function with conditional}

\medskip

\bigskip

Recursive definition using conditional expression:

\bigskip

\bigskip

viewed $\langle \rangle$ = $\langle \rangle$

\bigskip

\bigskip

viewed $\langle x \rangle$ ^ $s = if$ x.3 = yes then $\langle x \rangle$ ^ viewed s else viewed s

\bigskip

\bigskip
\noindent
\textbf{Solution 40 ( d ) - cumulative_total recursive function}

\medskip

\begin{axdef}
\mathit{cumulative\_total} : \seq~Title * Length * Viewed \fun \mathbb{N}
\where
\mathit{cumulative\_total}(\langle \rangle) = 0
\end{axdef}

\bigskip

Note: $\forall$ with semicolon-separated bindings not yet supported

\bigskip

\bigskip
\noindent
\textbf{Solution 41 ( c ) - 479_courses with conditional}

\medskip

\bigskip

$\forall$ $x : Entry$; $s : seq Entry |$

\bigskip

\bigskip

479_courses ($\langle \rangle$) = $\langle \rangle$

\bigskip

\bigskip

479_courses ($\langle x \rangle$ ^ s) = if x.3 = 479 then $\langle x \rangle$ ^ 479_courses s else 479_courses s

\bigskip

\bigskip
\noindent
\textbf{Solution 41 ( d ) - total function}

\medskip

\bigskip

$\forall$ $x : Entry$; $s : seq Entry |$

\bigskip

\bigskip

total ($\langle \rangle$) = 0

\bigskip

\bigskip

total ($\langle x \rangle$ ^ s) = x.5 + total s

\bigskip

\end{document}