\documentclass{article}
\usepackage{zed-cm}
\usepackage{zed-maths}
\usepackage{zed-proof}
\usepackage{amsmath}
\begin{document}

$$
\infer[\text{$\Rightarrow$ intro from 1}]{p \land (q \lor r) \Rightarrow p \land q \lor p \land r}{
  \infer[\text{$\lor$ elim}]{p \land q \lor p \land r}{\infer[\text{$\lor$ intro}]{p \land q \lor p \land r}{\infer[\text{$\land$ intro}]{p \land q}{\infer[\text{from above}]{p}{} & \infer[\text{from case}]{q}{}}} & \infer[\text{$\lor$ intro}]{p \land q \lor p \land r}{\infer[\text{$\land$ intro}]{p \land r}{\infer[\text{from above}]{p}{} & \infer[\text{from case}]{r}{}}}}
}
$$

\end{document}