\documentclass[a4paper,10pt,fleqn]{article}
\usepackage[margin=1in]{geometry}
\usepackage{amssymb}
\usepackage{adjustbox}
\usepackage{natbib}
\usepackage[colorlinks=true,linkcolor=blue,citecolor=blue,urlcolor=blue]{hyperref}
\usepackage{fuzz}
\usepackage{zed-maths}
\usepackage{zed-proof}
\newdimen\savedleftskip
\begin{document}

\begin{center}
  \adjustbox{max width=\textwidth}{%
    $\displaystyle
    \infer[\Rightarrow\textrm{-intro}^{[1]}]{p \land (q \lor r)
    \implies (p \land q) \lor (p \land r)}{
      \infer[\lor \mathrm{elim}]{(p \land q) \lor (p \land
      r)}{\infer[\lor\textrm{-intro-1}]{(p \land q) \lor (p \land
        r)}{\infer[\land \mathrm{intro}]{p \land
          q}{\infer[\mathrm{from} \mathrm{case}]{q}{\infer[\mathrm{from}
        above]{p}{}}}} & \infer[\lor\textrm{-intro-2}]{(p \land q) \lor
        (p \land r)}{\infer[\land \mathrm{intro}]{p \land
          r}{\infer[\mathrm{from} \mathrm{case}]{r}{\infer[\mathrm{from}
      above]{p}{}}}}}
    }
    $%
  }
\end{center}
\bigskip

\end{document}
